@prefix : <http://bioprotocols.org/paml#> .
@prefix opil: <http://bioprotocols.org/opil/v1#> .
@prefix om: <http://www.ontology-of-units-of-measure.org/resource/om-2/> .
@prefix owl: <http://www.w3.org/2002/07/owl#> .
@prefix rdf: <http://www.w3.org/1999/02/22-rdf-syntax-ns#> .
@prefix xml: <http://www.w3.org/XML/1998/namespace> .
@prefix xsd: <http://www.w3.org/2001/XMLSchema#> .
@prefix paml: <http://bioprotocols.org/paml#> .
@prefix rdfs: <http://www.w3.org/2000/01/rdf-schema#> .
@prefix sbol: <http://sbols.org/v3#> .
@prefix MathM: <http://www.w3.org/1998/Math/MathML> .
@base <http://bioprotocols.org/paml#> .

<http://bioprotocols.org/paml> rdf:type owl:Ontology ;
                              owl:imports sbol: ,
                                          om: ;
                              rdfs:comment "Protocol Activity Modeling Languge (PAML) ontology." ;
                              owl:versionInfo "0.3" .

#################################################################
#    Annotation properties
#################################################################

###  http://www.w3.org/2002/07/owl#maxCardinality
owl:maxCardinality rdf:type owl:AnnotationProperty .
owl:minCardinality rdf:type owl:AnnotationProperty .


#################################################################
#    Datatypes
#################################################################

###  http://www.w3.org/2001/XMLSchema#anySimpleType
xsd:anySimpleType rdf:type rdfs:Datatype .


#################################################################
#    Classes
#################################################################

# Activities (nodes)
paml:Activity rdf:type owl:Class ;
            rdfs:subClassOf sbol:Identified ;
              rdfs:comment "Activities are the nodes in an activity graph" .

paml:Control rdf:type owl:Class ;
        rdfs:subClassOf paml:Activity ;
              rdfs:comment "Abstract class; Control activities regulate progress through the activity graph" .
#       [ rdf:type owl:Restriction ;
#                owl:onProperty paml:controlType ;
#                owl:allValuesFrom xsd:anyURI
#                owl:minCardinality "1"^^xsd:nonNegativeInteger ;
#                owl:maxCardinality "1"^^xsd:nonNegativeInteger ;
#              ] ;
        
# change control subclasses can be changed into an enum on Control?
paml:Fork rdf:type owl:Class ;
        rdfs:subClassOf paml:Control ;
              rdfs:comment "Fork executes multiples paths in parallel" .

paml:Join rdf:type owl:Class ;
        rdfs:subClassOf paml:Control ;
              rdfs:comment "Join is the complement of Fork; it continues when ALL incoming flows are ready" .

paml:Initial rdf:type owl:Class ;
        rdfs:subClassOf paml:Fork ;
              rdfs:comment "Initial is a fork node that also initiates control flow through the network" .

paml:Final rdf:type owl:Class ;
        rdfs:subClassOf paml:Join ;
              rdfs:comment "Final is a join node that also terminates control flow through the network" .

paml:Decision rdf:type owl:Class ;
        rdfs:subClassOf paml:Control ;
              rdfs:comment "Decision is a branch that sends control flow to precisely one of the options." .

paml:Merge rdf:type owl:Class ;
        rdfs:subClassOf paml:Control ;
              rdfs:comment "Merge is the complement of Decision; it continues when ANY incoming flow is ready." .




paml:Executable rdf:type owl:Class ;
                rdfs:comment "Abstract class; executable activities manipulate flows of information or physical objects" ;
              rdfs:subClassOf paml:Activity ,
                              [ rdf:type owl:Restriction ;
                                  owl:onProperty paml:input ;
                                  owl:onClass paml:Pin
                                ] ,
                              [ rdf:type owl:Restriction ;
                                  owl:onProperty paml:output ;
                                 owl:onClass paml:Pin
                                ] .     
 
paml:Pin rdf:type owl:Class ;
       rdfs:subClassOf paml:Activity ;
         rdfs:comment "A Pin is a typed input or output of an Executable. Pins are Activities so that control can be applied to flows between them" ,
                              [ rdf:type owl:Restriction ;
                                  owl:onProperty paml:instanceOf ;
                                 owl:onClass paml:PinSpecification
                                ] .

# should the Value vs. Physical distinction be turned into a type rather than a class distinction?
paml:ValuePin rdf:type owl:Class ;
              rdfs:comment "A ValuePin represents information as an input or output" ;
            rdfs:subClassOf paml:Pin ,
                            [ rdf:type owl:Restriction ;
                                owl:onProperty paml:type ;
                                owl:allValuesFrom xsd:anyURI
                              ] .

paml:PhysicalPin rdf:type owl:Class ;
                 rdfs:comment "A PhysicalPin represents a physical input or output" ;
        rdfs:subClassOf paml:Pin ,
        [ rdf:type owl:Restriction ;
                owl:onProperty paml:type ;
                owl:onClass sbol:Component
              ] .

paml:PrimitiveExecutable rdf:type owl:Class ;
              rdfs:comment "An executable that is a base-level library function, with its Pins determined by the specification of the function" ;
        rdfs:subClassOf paml:Executable ,
        [ rdf:type owl:Restriction ;
                owl:onProperty paml:instanceOf ;
                owl:onClass paml:Primitive ;
                owl:minCardinality "1"^^xsd:nonNegativeInteger ;
                owl:maxCardinality "1"^^xsd:nonNegativeInteger ;
              ] .

paml:SubProtocol rdf:type owl:Class ;
              rdfs:comment "An executable that is implemented as a Protocol, with its Pins determined by the input and output properties" ;
        rdfs:subClassOf paml:Executable ,
        [ rdf:type owl:Restriction ;
                owl:onProperty paml:implementedBy ;
                owl:onClass paml:Protocol ;
                owl:minCardinality "1"^^xsd:nonNegativeInteger ;
                owl:maxCardinality "1"^^xsd:nonNegativeInteger ;
              ] .

paml:InformationExecutable rdf:type owl:Class ;
        rdfs:subClassOf paml:Executable ;
              rdfs:comment "Abstract class; Executable activities that interact only with information flows (i.e., has no PhysicalPin)" .

paml:PhysicalExecutable rdf:type owl:Class ;
        rdfs:subClassOf paml:Executable ;
              rdfs:comment "Abstract class; Executable activities that can interact with physical flows (i.e., has at least one PhysicalPin)" .


paml:Value rdf:type owl:Class ;
              rdfs:comment "Value activities are unilateral sources and sinks of information in the graph" ;
        rdfs:subClassOf paml:Activity ,
        [ rdf:type owl:Restriction ;
                owl:onProperty paml:type ;
                owl:allValuesFrom xsd:anyURI
              ] .

paml:Physical rdf:type owl:Class ;
              rdfs:comment "Physical activities are unilateral sources and sinks of physical materials in the graph" ;
        rdfs:subClassOf paml:Activity ,
        [ rdf:type owl:Restriction ;
                owl:onProperty paml:type ;
                owl:onClass sbol:Component
              ] .
        

# Flows (edges)
paml:Flow rdf:type owl:Class ;
              rdfs:comment "Flows are the edges of an activity graph" ;
              rdfs:comment "A flow connects precisely one activity source to precisely one activity sink" ;
              rdfs:subClassOf sbol:Identified ,
        [ rdf:type owl:Restriction ;
                owl:onProperty paml:source ;
                owl:minCardinality "1"^^xsd:nonNegativeInteger ;
                owl:maxCardinality "1"^^xsd:nonNegativeInteger ;
                owl:onClass paml:Activity
              ] ,
        [ rdf:type owl:Restriction ;
                owl:onProperty paml:sink ;
                owl:minCardinality "1"^^xsd:nonNegativeInteger ;
                owl:maxCardinality "1"^^xsd:nonNegativeInteger ;
                owl:onClass paml:Activity
              ] .

paml:source rdf:type owl:ObjectProperty ;
              rdfs:subPropertyOf opil:compositionalProperty ;
              rdfs:domain paml:Flow ;
              rdfs:range paml:Activity ;
              rdfs:label "source" ;
              rdfs:comment "Activity from which a flow originates" .

paml:sink rdf:type owl:ObjectProperty ;
              rdfs:subPropertyOf opil:compositionalProperty ;
              rdfs:domain paml:Flow ;
              rdfs:range paml:Activity ;
              rdfs:label "sink" ;
              rdfs:comment "Activity at which a flow arrives" .


paml:ControlFlow rdf:type owl:Class ;
        rdfs:subClassOf paml:Flow ;
              rdfs:comment "Control flows indicate that the source activity must occur before the sink activity" .

paml:InformationFlow rdf:type owl:Class ;
        rdfs:subClassOf paml:Flow ;
              rdfs:comment "Information flows indicate that information produced by an activity is used by another activity" .

paml:PhysicalFlow rdf:type owl:Class ;
        rdfs:subClassOf paml:Flow ;
              rdfs:comment "Physical flows indicate that a material produced by an activity is used by another activity" .


# Protocol
paml:Protocol rdf:type owl:Class ;
              rdfs:comment "A protocol is an acyclic directed graph made of activities (nodes) and flows (edges). It must have precisely one Initial and one Final that are the unique top and bottom nodes of the graph" ; 
        rdfs:subClassOf sbol:TopLevel ,
        [ rdf:type owl:Restriction ;
                owl:onProperty paml:hasActivity ;
                owl:onClass paml:Activity
              ] ,
        [ rdf:type owl:Restriction ;
                owl:onProperty paml:hasFlow ;
                owl:onClass paml:Flow
              ] ,
        [ rdf:type owl:Restriction ;
                owl:onProperty paml:input ;
                owl:onClass paml:Activity
              ] ,
        [ rdf:type owl:Restriction ;
                owl:onProperty paml:output ;
                owl:onClass paml:Activity ;
              rdfs:comment "Designation of an activity as an output of a Protocol"
              ] .

paml:hasActivity rdf:type owl:ObjectProperty ;
              rdfs:subPropertyOf opil:compositionalProperty ;
              rdfs:domain paml:Protocol ;
              rdfs:range paml:Activity ;
              rdfs:label "hasActivity" ;
              rdfs:comment "Activity in a Protocol" .

paml:hasFlow rdf:type owl:ObjectProperty ;
              rdfs:subPropertyOf opil:compositionalProperty ;
              rdfs:domain paml:Protocol ;
              rdfs:range paml:Flow ;
              rdfs:label "hasFlow" ;
              rdfs:comment "Flow in a Protocol" .

paml:input rdf:type owl:ObjectProperty ;
              rdfs:subPropertyOf opil:compositionalProperty ;
              rdfs:domain paml:Protocol ;
              rdfs:range paml:Activity ;
              rdfs:label "input" ;
              rdfs:comment "Designation of an activity as an input of a Protocol" .

paml:output rdf:type owl:ObjectProperty ;
              rdfs:subPropertyOf opil:compositionalProperty ;
              rdfs:label "output" ;
              rdfs:domain sbol:TopLevel ;
              rdfs:range sbol:Identified .

paml:Primitive rdf:type owl:Class ;
              rdfs:comment "An atomic protocol step, to be implemented by various platform-specific libraries" ;
        rdfs:subClassOf sbol:TopLevel ,
        [ rdf:type owl:Restriction ;
                owl:onProperty paml:input ;
                owl:onClass paml:PinSpecification
              ] ,
        [ rdf:type owl:Restriction ;
                owl:onProperty paml:output ;
                owl:onClass paml:PinSpecification
              ] .

#paml:input rdf:type owl:ObjectProperty ;
#              rdfs:subPropertyOf opil:compositionalProperty ;
#              rdfs:domain paml:Primitive ;
#              rdfs:range paml:PinSpecification ;
#              rdfs:label "input" ;
#              rdfs:comment "Specification for the input of a Primitive" .

#paml:output rdf:type owl:ObjectProperty ;
#              rdfs:subPropertyOf opil:compositionalProperty ;
#              rdfs:domain paml:Primitive ;
#              rdfs:range paml:PinSpecification ;
#              rdfs:label "hasActivity" ;
#              rdfs:comment "Specification for the output of a Primitive" .

paml:PinSpecification rdf:type owl:Class ;
              rdfs:comment "A ValuePin represents information as an input or output" ;
            rdfs:subClassOf sbol:Identified ,
                            [ rdf:type owl:Restriction ;
                                owl:onProperty sbol:name ;
                                owl:allValuesFrom xsd:string
                              ] ,
                            [ rdf:type owl:Restriction ;
                                owl:onProperty paml:type ;
                                owl:allValuesFrom xsd:anyURI
                              ] ,
                            [ rdf:type owl:Restriction ;
                                owl:onProperty paml:optional ;
                                owl:allValuesFrom xsd:boolean ;
                                rdfs:comment "Optional is not needed for output pins, which can always be ignored"
                              ] .


paml:Location rdf:type owl:Class ;
              rdfs:comment "Locations are containers, wells, etc." ;
            rdfs:subClassOf sbol:TopLevel .

paml:Microplate rdf:type owl:Class ;
              rdfs:comment "A standard well-array plate, such as a 96-well plate or 384-well plate" ;
        rdfs:subClassOf paml:Location .

paml:MicroplateWells rdf:type owl:Class ;
              rdfs:comment "A standard well-array plate, such as a 96-well plate or 384-well plate" ;
        rdfs:subClassOf paml:Location .
                            [ rdf:type owl:Restriction ;
                              owl:onProperty paml:plateCoordinates ;
                              owl:onClass xsd:string ;
                              rdfs:comment "Coordinates use Excel form, e.g., A1, B3:B6"
                              ] .
                            [ rdf:type owl:Restriction ;
                                owl:onProperty paml:inPlate ;
                                owl:onClass paml:Microplate
                              ] .

