@prefix owl: <http://www.w3.org/2002/07/owl#> .
@prefix rdfs: <http://www.w3.org/2000/01/rdf-schema#> .
@prefix sbol: <http://sbols.org/v3#> .
@prefix uml: <http://bioprotocols.org/uml#> .
@prefix xsd: <http://www.w3.org/2001/XMLSchema#> .

<http://bioprotocols.org/uml> a owl:Ontology ;
    rdfs:comment "Unified Modeling Languge (UML) subset, translated to an SBOL factory ontology." ;
    owl:imports <http://sbols.org/v3>,
        <http://www.ontology-of-units-of-measure.org/resource/om-2> ;
    owl:versionInfo "1.0-alpha1" .

uml:ControlFlow a owl:Class ;
    rdfs:comment "A ControlFlow is an ActivityEdge traversed by control tokens or object tokens of control type, which are use to control the execution of ExecutableNodes. See UML 2.5.1 specification section 15.2." ;
    rdfs:subClassOf uml:ActivityEdge .

uml:FlowFinalNode a owl:Class ;
    rdfs:comment "A FlowFinalNode is a FinalNode that terminates a flow. All tokens accepted by a FlowFinalNode are destroyed. This has no effect on other flows in the Activity. See UML 2.5.1 specification section 15.3." ;
    rdfs:subClassOf uml:FinalNode .

uml:ForkNode a owl:Class ;
    rdfs:comment "A ForkNode is a ControlNode that splits a flow into multiple concurrent flows. A ForkNode shall have exactly one incoming ActivityEdge, though it may have multiple outgoing ActivityEdges. See UML 2.5.1 specification section 15.3." ;
    rdfs:subClassOf uml:ControlNode .

uml:InitialNode a owl:Class ;
    rdfs:comment "An InitialNode acts as a starting point for executing an Activity. An Activity may have more than one InitialNodes that start multiple concurrent control flows. See UML 2.5.1 specification section 15.3." ;
    rdfs:subClassOf uml:ControlNode .

uml:JoinNode a owl:Class ;
    rdfs:comment "A JoinNode is a ControlNode that synchronizes multiple flows. A JoinNode shall have exactly one outgoing ActivityEdge but may have multiple incoming ActivityEdges. See UML 2.5.1 specification section 15.3." ;
    rdfs:subClassOf uml:ControlNode .

uml:LiteralNull a owl:Class ;
    rdfs:comment "A LiteralNull specifies the lack of a value. See UML 2.5.1 specification section 8.2." ;
    rdfs:subClassOf uml:LiteralSpecification .

uml:MergeNode a owl:Class ;
    rdfs:comment "A MergeNode is a control node that brings together multiple flows without synchronization. A MergeNode shall have exactly one outgoing ActivityEdge but may have multiple incoming ActivityEdges. See UML 2.5.1 specification section 15.3." ;
    rdfs:subClassOf uml:ControlNode .

xsd:anySimpleType a rdfs:Datatype .

uml:ActivityParameterNode a owl:Class ;
    rdfs:comment "An ActivityParameterNode is an ObjectNode for accepting values from the input Parameters or providing values to the output Parameters of an Activity. UML 2.5.1 specification section 15.4." ;
    rdfs:subClassOf [ a owl:Restriction ;
            owl:allValuesFrom uml:OrderedPropertyValue ;
            owl:onProperty uml:parameter ],
        [ a owl:Restriction ;
            owl:minCardinality "1"^^xsd:nonNegativeInteger ;
            owl:onProperty uml:parameter ],
        [ a owl:Restriction ;
            owl:maxCardinality "1"^^xsd:nonNegativeInteger ;
            owl:onProperty uml:parameter ],
        uml:ObjectNode .

uml:CallAction a owl:Class ;
    rdfs:comment "A CallAction is an abstract class for Actions that invoke a Behavior with given argument values and (if the invocation is synchronous) receive reply values. See UML 2.5.1 specification section 16.3." ;
    rdfs:subClassOf uml:InvocationAction .

uml:CallBehaviorAction a owl:Class ;
    rdfs:comment "A CallBehaviorAction is a CallAction that invokes a Behavior directly. The argument values of the CallBehaviorAction are passed on the input Parameters of the invoked Behavior. UML 2.5.1 specification section 16.3" ;
    rdfs:subClassOf [ a owl:Restriction ;
            owl:allValuesFrom uml:Behavior ;
            owl:onProperty uml:behavior ],
        [ a owl:Restriction ;
            owl:minCardinality "1"^^xsd:nonNegativeInteger ;
            owl:onProperty uml:behavior ],
        [ a owl:Restriction ;
            owl:maxCardinality "1"^^xsd:nonNegativeInteger ;
            owl:onProperty uml:behavior ],
        uml:CallAction .

uml:ExecutableNode a owl:Class ;
    rdfs:comment "An ExecutableNode is an abstract class for ActivityNodes whose execution may be controlled using ControlFlows and to which ExceptionHandlers may be attached. See UML 2.5.1 specification section 15.5." ;
    rdfs:subClassOf uml:ActivityNode .

uml:FinalNode a owl:Class ;
    rdfs:comment "A FinalNode is a ControlNode at which a flow in an Activity stops. A FinalNode shall not have outgoing ActivityEdges. See UML 2.5.1 specification section 15.3." ;
    rdfs:subClassOf uml:ControlNode .

uml:InvocationAction a owl:Class ;
    rdfs:comment "UML 2.5.1 specification section 16.3" ;
    rdfs:subClassOf uml:Action .

uml:LiteralBoolean a owl:Class ;
    rdfs:comment "A LiteralBoolean is a specification of a Boolean value. See UML 2.5.1 specification section 8.2." ;
    rdfs:subClassOf [ a owl:Restriction ;
            owl:allValuesFrom xsd:boolean ;
            owl:onProperty uml:booleanValue ],
        [ a owl:Restriction ;
            owl:minCardinality "1"^^xsd:nonNegativeInteger ;
            owl:onProperty uml:booleanValue ],
        [ a owl:Restriction ;
            owl:maxCardinality "1"^^xsd:nonNegativeInteger ;
            owl:onProperty uml:booleanValue ],
        uml:LiteralSpecification .

uml:LiteralIdentified a owl:Class ;
    rdfs:comment "A LiteralIdentified is used for linking SBOL objects as a child object to UML objects." ;
    rdfs:subClassOf [ a owl:Restriction ;
            owl:allValuesFrom sbol:Identified ;
            owl:onProperty uml:identifiedValue ],
        [ a owl:Restriction ;
            owl:minCardinality "1"^^xsd:nonNegativeInteger ;
            owl:onProperty uml:identifiedValue ],
        [ a owl:Restriction ;
            owl:maxCardinality "1"^^xsd:nonNegativeInteger ;
            owl:onProperty uml:identifiedValue ],
        uml:LiteralSpecification .

uml:LiteralInteger a owl:Class ;
    rdfs:comment "A LiteralInteger is a specification of an Integer value. See UML 2.5.1 specification section 8.2." ;
    rdfs:subClassOf [ a owl:Restriction ;
            owl:allValuesFrom xsd:integer ;
            owl:onProperty uml:integerValue ],
        [ a owl:Restriction ;
            owl:minCardinality "1"^^xsd:nonNegativeInteger ;
            owl:onProperty uml:integerValue ],
        [ a owl:Restriction ;
            owl:maxCardinality "1"^^xsd:nonNegativeInteger ;
            owl:onProperty uml:integerValue ],
        uml:LiteralSpecification .

uml:LiteralReal a owl:Class ;
    rdfs:comment "A LiteralReal is a specification of a Real value. See UML 2.5.1 specification section 8.2." ;
    rdfs:subClassOf [ a owl:Restriction ;
            owl:allValuesFrom xsd:float ;
            owl:onProperty uml:realValue ],
        [ a owl:Restriction ;
            owl:minCardinality "1"^^xsd:nonNegativeInteger ;
            owl:onProperty uml:realValue ],
        [ a owl:Restriction ;
            owl:maxCardinality "1"^^xsd:nonNegativeInteger ;
            owl:onProperty uml:realValue ],
        uml:LiteralSpecification .

uml:LiteralReference a owl:Class ;
    rdfs:comment "A LiteralReference is used for embedding SBOL objects as a reference." ;
    rdfs:subClassOf [ a owl:Restriction ;
            owl:maxCardinality "1"^^xsd:nonNegativeInteger ;
            owl:onProperty uml:referenceValue ],
        [ a owl:Restriction ;
            owl:allValuesFrom sbol:Identified ;
            owl:onProperty uml:referenceValue ],
        [ a owl:Restriction ;
            owl:minCardinality "1"^^xsd:nonNegativeInteger ;
            owl:onProperty uml:referenceValue ],
        uml:LiteralSpecification .

uml:LiteralString a owl:Class ;
    rdfs:comment "A LiteralSpecification identifies a literal constant being modeled. See UML 2.5.1 specification section 8.2." ;
    rdfs:subClassOf [ a owl:Restriction ;
            owl:allValuesFrom xsd:string ;
            owl:onProperty uml:stringValue ],
        [ a owl:Restriction ;
            owl:minCardinality "1"^^xsd:nonNegativeInteger ;
            owl:onProperty uml:stringValue ],
        [ a owl:Restriction ;
            owl:maxCardinality "1"^^xsd:nonNegativeInteger ;
            owl:onProperty uml:stringValue ],
        uml:LiteralSpecification .

uml:ValuePin a owl:Class ;
    rdfs:comment "A ValuePin is an InputPin that provides a value by evaluating a ValueSpecification. See UML 2.5.1 specification section 16.2." ;
    rdfs:subClassOf [ a owl:Restriction ;
            owl:allValuesFrom uml:ValueSpecification ;
            owl:onProperty uml:value ],
        [ a owl:Restriction ;
            owl:minCardinality "1"^^xsd:nonNegativeInteger ;
            owl:onProperty uml:value ],
        [ a owl:Restriction ;
            owl:maxCardinality "1"^^xsd:nonNegativeInteger ;
            owl:onProperty uml:value ],
        uml:InputPin .

uml:constrainedElement a owl:ObjectProperty ;
    rdfs:label "constrained_elements" ;
    rdfs:comment "The OrderedPropertyValue referenced by this Constraint." ;
    rdfs:domain uml:Constraint ;
    rdfs:range uml:OrderedPropertyValue ;
    rdfs:subPropertyOf sbol:directlyComprises .

uml:edge a owl:ObjectProperty ;
    rdfs:label "edges" ;
    rdfs:comment "ActivityEdges expressing flow between the nodes of the Activity." ;
    rdfs:domain uml:Activity ;
    rdfs:range uml:ActivityEdge ;
    rdfs:subPropertyOf sbol:directlyComprises .

uml:input a owl:ObjectProperty ;
    rdfs:label "inputs" ;
    rdfs:comment "The ordered set of InputPins representing the inputs to the Action." ;
    rdfs:domain uml:Action ;
    rdfs:range uml:InputPin ;
    rdfs:subPropertyOf sbol:directlyComprises .

uml:node a owl:ObjectProperty ;
    rdfs:label "nodes" ;
    rdfs:comment "ActivityNodes coordinated by the Activity." ;
    rdfs:domain uml:Activity ;
    rdfs:range uml:ActivityNode ;
    rdfs:subPropertyOf sbol:directlyComprises .

uml:operandValue a owl:ObjectProperty ;
    rdfs:label "operand" ;
    rdfs:comment "Specifies a sequence of operand ValueSpecifications." ;
    rdfs:domain uml:Expression ;
    rdfs:range uml:OrderedPropertyValue ;
    rdfs:subPropertyOf sbol:directlyComprises .

uml:output a owl:ObjectProperty ;
    rdfs:label "outputs" ;
    rdfs:comment "The ordered set of OutputPins representing outputs from the Action." ;
    rdfs:domain uml:Action ;
    rdfs:range uml:OutputPin ;
    rdfs:subPropertyOf sbol:directlyComprises .

uml:ownedParameter a owl:ObjectProperty ;
    rdfs:label "parameters" ;
    rdfs:comment " a list of Parameters to the Behavior which describes the order and type of arguments that can be given when the Behavior is invoked and of the values which will be returned when the Behavior completes its execution." ;
    rdfs:domain uml:Behavior ;
    rdfs:range uml:OrderedPropertyValue ;
    rdfs:subPropertyOf sbol:directlyComprises .

uml:postcondition a owl:ObjectProperty ;
    rdfs:label "postconditions" ;
    rdfs:comment "An optional set of Constraints specifying what is fulfilled after the execution of the Behavior is completed, if its precondition was fulfilled before its invocation." ;
    rdfs:domain uml:Behavior ;
    rdfs:range uml:Constraint ;
    rdfs:subPropertyOf sbol:directlyComprises .

uml:precondition a owl:ObjectProperty ;
    rdfs:label "preconditions" ;
    rdfs:comment "An optional set of Constraints specifying what must be fulfilled before the Behavior is invoked." ;
    rdfs:domain uml:Behavior ;
    rdfs:range uml:Constraint ;
    rdfs:subPropertyOf sbol:directlyComprises .

uml:Activity a owl:Class ;
    rdfs:comment "An Activity coordinates and groups steps in a protocol or workflow. See UML 2.5.1 specification section 15." ;
    rdfs:subClassOf [ a owl:Restriction ;
            owl:allValuesFrom uml:ActivityNode ;
            owl:onProperty uml:node ],
        [ a owl:Restriction ;
            owl:allValuesFrom uml:ActivityEdge ;
            owl:onProperty uml:edge ],
        uml:Behavior .

uml:DecisionNode a owl:Class ;
    rdfs:comment "A DecisionNode is a ControlNode that chooses between outgoing flows. A DecisionNode shall have at least one and at most two incoming ActivityEdges, and at least one outgoing ActivityEdge. See UML 2.5.1 specification section 15.3." ;
    rdfs:subClassOf [ a owl:Restriction ;
            owl:allValuesFrom uml:Behavior ;
            owl:onProperty uml:decisionInput ],
        [ a owl:Restriction ;
            owl:maxCardinality "1"^^xsd:nonNegativeInteger ;
            owl:onProperty uml:decisionInput ],
        [ a owl:Restriction ;
            owl:allValuesFrom uml:ObjectFlow ;
            owl:onProperty uml:decisionInputFlow ],
        [ a owl:Restriction ;
            owl:maxCardinality "1"^^xsd:nonNegativeInteger ;
            owl:onProperty uml:decisionInputFlow ],
        uml:ControlNode .

uml:DurationConstraint a owl:Class ;
    rdfs:comment "A DurationConstraint is a Constraint that refers to a DurationInterval." ;
    rdfs:subClassOf [ a owl:Restriction ;
            owl:maxCardinality "2"^^xsd:nonNegativeInteger ;
            owl:onProperty uml:firstEventValue ],
        [ a owl:Restriction ;
            owl:maxCardinality "1"^^xsd:nonNegativeInteger ;
            owl:onProperty uml:durationSpecification ],
        [ a owl:Restriction ;
            owl:minCardinality "1"^^xsd:nonNegativeInteger ;
            owl:onProperty uml:durationSpecification ],
        [ a owl:Restriction ;
            owl:minCardinality "0"^^xsd:nonNegativeInteger ;
            owl:onProperty uml:firstEventValue ],
        [ a owl:Restriction ;
            owl:allValuesFrom uml:OrderedPropertyValue ;
            owl:onProperty uml:firstEventValue ],
        uml:IntervalConstraint .

uml:DurationObservation a owl:Class ;
    rdfs:comment "A DurationObservation is a reference to a duration during an execution. It points out the entities in the model to observe and whether the observations are when these entities are entered or exited." ;
    rdfs:subClassOf [ a owl:Restriction ;
            owl:minCardinality "1"^^xsd:nonNegativeInteger ;
            owl:onProperty uml:durationObservationValue ],
        [ a owl:Restriction ;
            owl:allValuesFrom sbol:Identified ;
            owl:onProperty uml:durationObservationValue ],
        [ a owl:Restriction ;
            owl:allValuesFrom uml:OrderedPropertyValue ;
            owl:onProperty uml:firstEventValue ],
        [ a owl:Restriction ;
            owl:minCardinality "0"^^xsd:nonNegativeInteger ;
            owl:onProperty uml:firstEventValue ],
        [ a owl:Restriction ;
            owl:maxCardinality "2"^^xsd:nonNegativeInteger ;
            owl:onProperty uml:firstEventValue ],
        [ a owl:Restriction ;
            owl:maxCardinality "2"^^xsd:nonNegativeInteger ;
            owl:onProperty uml:durationObservationValue ],
        uml:Observation .

uml:Expression a owl:Class ;
    rdfs:comment "An Expression represents a node in an expression tree, which may be non-terminal or terminal. It defines a symbol, and has a possibly empty sequence of operands that are ValueSpecifications. See UML 2.5.1 specification section 8.6.5.1." ;
    rdfs:subClassOf [ a owl:Restriction ;
            owl:minCardinality "1"^^xsd:nonNegativeInteger ;
            owl:onProperty uml:isOrdered ],
        [ a owl:Restriction ;
            owl:allValuesFrom xsd:boolean ;
            owl:onProperty uml:isOrdered ],
        [ a owl:Restriction ;
            owl:minCardinality "0"^^xsd:nonNegativeInteger ;
            owl:onProperty uml:symbolValue ],
        [ a owl:Restriction ;
            owl:maxCardinality "1"^^xsd:nonNegativeInteger ;
            owl:onProperty uml:symbolValue ],
        [ a owl:Restriction ;
            owl:maxCardinality "1"^^xsd:nonNegativeInteger ;
            owl:onProperty uml:isOrdered ],
        [ a owl:Restriction ;
            owl:allValuesFrom xsd:string ;
            owl:onProperty uml:symbolValue ],
        [ a owl:Restriction ;
            owl:allValuesFrom uml:OrderedPropertyValue ;
            owl:onProperty uml:operandValue ],
        uml:ValueSpecification .

uml:Interval a owl:Class ;
    rdfs:comment "An Interval defines the range between two ValueSpecifications." ;
    rdfs:subClassOf uml:ValueSpecification .

uml:IntervalConstraint a owl:Class ;
    rdfs:comment "An IntervalConstraint is a Constraint that is specified by an Interval." ;
    rdfs:subClassOf uml:Constraint .

uml:ObjectFlow a owl:Class ;
    rdfs:comment "An ObjectFlow is an ActivityEdge that is traversed by object tokens that may hold values. Object flows also support multicast/receive, token selection from object nodes, and transformation of tokens. See UML 2.5.1 specification section 15.2." ;
    rdfs:subClassOf uml:ActivityEdge .

uml:ObjectNode a owl:Class ;
    rdfs:comment "An ObjectNode is a kind of ActivityNode used to hold value-containing object tokens during the course of the execution of an Activity. See UML 2.5.1 specification section 15.4." ;
    rdfs:subClassOf [ a owl:Restriction ;
            owl:allValuesFrom xsd:anyURI ;
            owl:onProperty uml:type ],
        [ a owl:Restriction ;
            owl:maxCardinality "1"^^xsd:nonNegativeInteger ;
            owl:onProperty uml:type ],
        uml:ActivityNode .

uml:OutputPin a owl:Class ;
    rdfs:comment "An OutputPin is a Pin that holds output values produced by an Action. See UML 2.5.1 specification section 16.2." ;
    rdfs:subClassOf uml:Pin .

uml:Parameter a owl:Class ;
    rdfs:comment "A Parameter is a specification of an argument used to pass information into or out of an invocation of a Behavior. See UML 2.5.1 specification section 9.4." ;
    rdfs:subClassOf [ a owl:Restriction ;
            owl:allValuesFrom xsd:anyURI ;
            owl:onProperty uml:direction ],
        [ a owl:Restriction ;
            owl:minCardinality "1"^^xsd:nonNegativeInteger ;
            owl:onProperty uml:direction ],
        [ a owl:Restriction ;
            owl:maxCardinality "1"^^xsd:nonNegativeInteger ;
            owl:onProperty uml:direction ],
        [ a owl:Restriction ;
            owl:allValuesFrom uml:ValueSpecification ;
            owl:onProperty uml:defaultValue ],
        [ a owl:Restriction ;
            owl:maxCardinality "1"^^xsd:nonNegativeInteger ;
            owl:onProperty uml:defaultValue ],
        [ a owl:Restriction ;
            owl:allValuesFrom xsd:anyURI ;
            owl:onProperty uml:type ],
        [ a owl:Restriction ;
            owl:maxCardinality "1"^^xsd:nonNegativeInteger ;
            owl:onProperty uml:type ],
        [ a owl:Restriction ;
            owl:allValuesFrom xsd:boolean ;
            owl:onProperty uml:isOrdered ],
        [ a owl:Restriction ;
            owl:minCardinality "1"^^xsd:nonNegativeInteger ;
            owl:onProperty uml:isOrdered ],
        [ a owl:Restriction ;
            owl:maxCardinality "1"^^xsd:nonNegativeInteger ;
            owl:onProperty uml:isOrdered ],
        [ a owl:Restriction ;
            owl:allValuesFrom xsd:boolean ;
            owl:onProperty uml:isUnique ],
        [ a owl:Restriction ;
            owl:minCardinality "1"^^xsd:nonNegativeInteger ;
            owl:onProperty uml:isUnique ],
        [ a owl:Restriction ;
            owl:maxCardinality "1"^^xsd:nonNegativeInteger ;
            owl:onProperty uml:isUnique ],
        [ a owl:Restriction ;
            owl:allValuesFrom uml:ValueSpecification ;
            owl:onProperty uml:lowerValue ],
        [ a owl:Restriction ;
            owl:maxCardinality "1"^^xsd:nonNegativeInteger ;
            owl:onProperty uml:lowerValue ],
        [ a owl:Restriction ;
            owl:allValuesFrom uml:ValueSpecification ;
            owl:onProperty uml:upperValue ],
        [ a owl:Restriction ;
            owl:maxCardinality "1"^^xsd:nonNegativeInteger ;
            owl:onProperty uml:upperValue ],
        sbol:Identified .

uml:Pin a owl:Class ;
    rdfs:comment "A Pin is an ObjectNode and MultiplicityElement that provides input values to an Action or accepts output values from an Action. See UML 2.5.1 specification section 16.2." ;
    rdfs:subClassOf [ a owl:Restriction ;
            owl:allValuesFrom xsd:boolean ;
            owl:onProperty uml:isOrdered ],
        [ a owl:Restriction ;
            owl:minCardinality "1"^^xsd:nonNegativeInteger ;
            owl:onProperty uml:isOrdered ],
        [ a owl:Restriction ;
            owl:maxCardinality "1"^^xsd:nonNegativeInteger ;
            owl:onProperty uml:isOrdered ],
        [ a owl:Restriction ;
            owl:allValuesFrom xsd:boolean ;
            owl:onProperty uml:isUnique ],
        [ a owl:Restriction ;
            owl:minCardinality "1"^^xsd:nonNegativeInteger ;
            owl:onProperty uml:isUnique ],
        [ a owl:Restriction ;
            owl:maxCardinality "1"^^xsd:nonNegativeInteger ;
            owl:onProperty uml:isUnique ],
        [ a owl:Restriction ;
            owl:allValuesFrom uml:ValueSpecification ;
            owl:onProperty uml:lowerValue ],
        [ a owl:Restriction ;
            owl:maxCardinality "1"^^xsd:nonNegativeInteger ;
            owl:onProperty uml:lowerValue ],
        [ a owl:Restriction ;
            owl:allValuesFrom uml:ValueSpecification ;
            owl:onProperty uml:upperValue ],
        [ a owl:Restriction ;
            owl:maxCardinality "1"^^xsd:nonNegativeInteger ;
            owl:onProperty uml:upperValue ],
        uml:ObjectNode .

uml:TimeConstraint a owl:Class ;
    rdfs:comment "A TimeConstraint is a Constraint that refers to a TimeInterval." ;
    rdfs:subClassOf [ a owl:Restriction ;
            owl:maxCardinality "1"^^xsd:nonNegativeInteger ;
            owl:onProperty uml:timeSpecification ],
        [ a owl:Restriction ;
            owl:maxCardinality "1"^^xsd:nonNegativeInteger ;
            owl:onProperty uml:firstEventValue ],
        [ a owl:Restriction ;
            owl:minCardinality "0"^^xsd:nonNegativeInteger ;
            owl:onProperty uml:firstEventValue ],
        [ a owl:Restriction ;
            owl:minCardinality "1"^^xsd:nonNegativeInteger ;
            owl:onProperty uml:timeSpecification ],
        [ a owl:Restriction ;
            owl:allValuesFrom uml:OrderedPropertyValue ;
            owl:onProperty uml:firstEventValue ],
        uml:IntervalConstraint .

uml:TimeObservation a owl:Class ;
    rdfs:comment "A TimeObservation is a reference to a time instant during an execution. It points out which entity in the model to observe and whether the observation is when this entity is entered or when it is exited." ;
    rdfs:subClassOf [ a owl:Restriction ;
            owl:maxCardinality "1"^^xsd:nonNegativeInteger ;
            owl:onProperty uml:timeObservationValue ],
        [ a owl:Restriction ;
            owl:minCardinality "1"^^xsd:nonNegativeInteger ;
            owl:onProperty uml:timeObservationValue ],
        [ a owl:Restriction ;
            owl:maxCardinality "1"^^xsd:nonNegativeInteger ;
            owl:onProperty uml:firstEventValue ],
        [ a owl:Restriction ;
            owl:allValuesFrom sbol:Identified ;
            owl:onProperty uml:timeObservationValue ],
        [ a owl:Restriction ;
            owl:allValuesFrom uml:OrderedPropertyValue ;
            owl:onProperty uml:firstEventValue ],
        [ a owl:Restriction ;
            owl:minCardinality "1"^^xsd:nonNegativeInteger ;
            owl:onProperty uml:firstEventValue ],
        uml:Observation .

uml:decisionInput a owl:ObjectProperty ;
    rdfs:label "decision_input" ;
    rdfs:comment "A Behavior that is executed to provide an input to guard ValueSpecifications on ActivityEdges outgoing from the DecisionNode." ;
    rdfs:domain uml:DecisionNode ;
    rdfs:range uml:Behavior .

uml:decisionInputFlow a owl:ObjectProperty ;
    rdfs:label "decision_input_flow" ;
    rdfs:comment "An additional ActivityEdge incoming to the DecisionNode that provides a decision input value for the guards ValueSpecifications on ActivityEdges outgoing from the DecisionNode." ;
    rdfs:domain uml:DecisionNode ;
    rdfs:range uml:ObjectFlow .

uml:defaultValue a owl:ObjectProperty ;
    rdfs:label "default_value" ;
    rdfs:comment "A ValueSpecification that represents a value to be used when no argument is supplied for the Parameter." ;
    rdfs:domain uml:Parameter ;
    rdfs:range uml:ValueSpecification ;
    rdfs:subPropertyOf sbol:directlyComprises .

uml:observationValue a owl:ObjectProperty ;
    rdfs:label "observation" ;
    rdfs:comment "Refers to the Observations that are involved in the computation of the Duration value." ;
    rdfs:domain uml:Duration,
        uml:TimeExpression ;
    rdfs:range uml:Observation .

uml:Action a owl:Class ;
    rdfs:comment "An Action is the fundamental unit of executable functionality. The execution of an Action represents some transformation or processing in the modeled system. Actions provide the ExecutableNodes within Activities and may also be used within Interactions. See UML 2.5.1 specification section 16." ;
    rdfs:subClassOf [ a owl:Restriction ;
            owl:allValuesFrom uml:InputPin ;
            owl:onProperty uml:input ],
        [ a owl:Restriction ;
            owl:allValuesFrom uml:OutputPin ;
            owl:onProperty uml:output ],
        uml:ExecutableNode .

uml:InputPin a owl:Class ;
    rdfs:comment "An InputPin is a Pin that holds input values to be consumed by an Action. See UML 2.5.1 specification section 16.2." ;
    rdfs:subClassOf uml:Pin .

uml:behavior a owl:ObjectProperty ;
    rdfs:label "behavior" ;
    rdfs:comment "The Behavior being invoked." ;
    rdfs:domain uml:CallBehaviorAction ;
    rdfs:range uml:Behavior .

uml:booleanValue a owl:DatatypeProperty ;
    rdfs:label "value" ;
    rdfs:comment "The specified Boolean value." ;
    rdfs:domain uml:LiteralBoolean ;
    rdfs:range xsd:boolean .

uml:direction a owl:DatatypeProperty ;
    rdfs:label "direction" ;
    rdfs:comment "Indicates whether a parameter is being sent into or out of a behavioral element." ;
    rdfs:domain uml:Parameter ;
    rdfs:range xsd:anyURI .

uml:durationObservationValue a owl:ObjectProperty ;
    rdfs:label "event" ;
    rdfs:comment "The DurationObservation is determined as the duration between the entering or exiting of a single event during execution, or the entering/exiting of one event and the entering/exiting of a second." ;
    rdfs:domain uml:DurationObservation ;
    rdfs:range sbol:Identified .

uml:durationSpecification a owl:ObjectProperty ;
    rdfs:label "specification" ;
    rdfs:comment "The DurationInterval constraining the duration." ;
    rdfs:domain uml:DurationConstraint ;
    rdfs:range uml:DurationInterval ;
    rdfs:subPropertyOf sbol:directlyComprises .

uml:identifiedValue a owl:ObjectProperty ;
    rdfs:label "value" ;
    rdfs:comment "The embedded SBOL object" ;
    rdfs:domain uml:LiteralIdentified ;
    rdfs:range sbol:Identified ;
    rdfs:subPropertyOf sbol:directlyComprises .

uml:indexValue a owl:DatatypeProperty ;
    rdfs:label "index" ;
    rdfs:domain uml:OrderedPropertyValue ;
    rdfs:range xsd:integer .

uml:integerValue a owl:DatatypeProperty ;
    rdfs:label "value" ;
    rdfs:comment "The specified Integer value." ;
    rdfs:domain uml:LiteralInteger ;
    rdfs:range xsd:integer .

uml:maxDurationValue a owl:ObjectProperty ;
    rdfs:label "max" ;
    rdfs:comment "Refers to the Duration denoting the maximum value of the range." ;
    rdfs:domain uml:DurationInterval ;
    rdfs:range uml:Duration ;
    rdfs:subPropertyOf sbol:directlyComprises .

uml:maxTimeValue a owl:ObjectProperty ;
    rdfs:label "max" ;
    rdfs:comment "Refers to the TimeExpression denoting the maximum value of the range." ;
    rdfs:domain uml:TimeInterval ;
    rdfs:range uml:TimeExpression ;
    rdfs:subPropertyOf sbol:directlyComprises .

uml:minDurationValue a owl:ObjectProperty ;
    rdfs:label "min" ;
    rdfs:comment "Refers to the Duration denoting the minimum value of the range." ;
    rdfs:domain uml:DurationInterval ;
    rdfs:range uml:Duration ;
    rdfs:subPropertyOf sbol:directlyComprises .

uml:minTimeValue a owl:ObjectProperty ;
    rdfs:label "min" ;
    rdfs:comment "Refers to the TimeExpression denoting the minimum value of the range." ;
    rdfs:domain uml:TimeInterval ;
    rdfs:range uml:TimeExpression ;
    rdfs:subPropertyOf sbol:directlyComprises .

uml:parameter a owl:ObjectProperty ;
    rdfs:label "parameter" ;
    rdfs:comment "The Parameter for which the ActivityParameterNode will be accepting or providing values." ;
    rdfs:domain uml:ActivityParameterNode ;
    rdfs:range uml:OrderedPropertyValue .

uml:propertyValue a owl:ObjectProperty ;
    rdfs:label "property_value" ;
    rdfs:domain uml:OrderedPropertyValue ;
    rdfs:range sbol:Identified ;
    rdfs:subPropertyOf sbol:directlyComprises .

uml:realValue a owl:DatatypeProperty ;
    rdfs:label "value" ;
    rdfs:comment "The specified Real value." ;
    rdfs:domain uml:LiteralReal ;
    rdfs:range xsd:float .

uml:referenceValue a owl:ObjectProperty ;
    rdfs:label "value" ;
    rdfs:comment "The referenced SBOL object." ;
    rdfs:domain uml:LiteralReference ;
    rdfs:range sbol:Identified .

uml:source a owl:ObjectProperty ;
    rdfs:label "source" ;
    rdfs:comment "The ActivityNode from which tokens are taken when they traverse the ActivityEdge." ;
    rdfs:domain uml:ActivityEdge ;
    rdfs:range uml:ActivityNode .

uml:stringValue a owl:DatatypeProperty ;
    rdfs:label "value" ;
    rdfs:comment "The specified String value." ;
    rdfs:domain uml:LiteralString ;
    rdfs:range xsd:string .

uml:symbolValue a owl:DatatypeProperty ;
    rdfs:label "symbol" ;
    rdfs:comment "The symbol associated with this node in the expression tree." ;
    rdfs:domain uml:Expression ;
    rdfs:range xsd:anyURI .

uml:target a owl:ObjectProperty ;
    rdfs:label "target" ;
    rdfs:comment "The ActivityNode to which tokens are put when they traverse the ActivityEdge." ;
    rdfs:domain uml:ActivityEdge ;
    rdfs:range uml:ActivityNode .

uml:timeObservationValue a owl:ObjectProperty ;
    rdfs:label "event" ;
    rdfs:comment "The TimeObservation is determined by the entering or exiting of the event during execution." ;
    rdfs:domain uml:TimeObservation ;
    rdfs:range sbol:Identified .

uml:timeSpecification a owl:ObjectProperty ;
    rdfs:label "specification" ;
    rdfs:comment "TheTimeInterval constraining the duration." ;
    rdfs:domain uml:TimeConstraint ;
    rdfs:range uml:TimeInterval ;
    rdfs:subPropertyOf sbol:directlyComprises .

uml:value a owl:ObjectProperty ;
    rdfs:label "value" ;
    rdfs:comment "The ValueSpecification that is evaluated to obtain the value that the ValuePin will provide." ;
    rdfs:domain uml:ValuePin ;
    rdfs:range uml:ValueSpecification ;
    rdfs:subPropertyOf sbol:directlyComprises .

uml:Duration a owl:Class ;
    rdfs:comment "A Duration is a ValueSpecification that specifies the temporal distance between two time instants." ;
    rdfs:subClassOf [ a owl:Restriction ;
            owl:maxCardinality "1"^^xsd:nonNegativeInteger ;
            owl:onProperty uml:exprValue ],
        [ a owl:Restriction ;
            owl:allValuesFrom uml:ValueSpecification ;
            owl:onProperty uml:exprValue ],
        [ a owl:Restriction ;
            owl:minCardinality "0"^^xsd:nonNegativeInteger ;
            owl:onProperty uml:exprValue ],
        [ a owl:Restriction ;
            owl:allValuesFrom uml:Observation ;
            owl:onProperty uml:observationValue ],
        uml:ValueSpecification .

uml:DurationInterval a owl:Class ;
    rdfs:comment "A DurationInterval defines the range between two Durations." ;
    rdfs:subClassOf [ a owl:Restriction ;
            owl:maxCardinality "1"^^xsd:nonNegativeInteger ;
            owl:onProperty uml:maxDurationValue ],
        [ a owl:Restriction ;
            owl:maxCardinality "1"^^xsd:nonNegativeInteger ;
            owl:onProperty uml:minDurationValue ],
        [ a owl:Restriction ;
            owl:minCardinality "1"^^xsd:nonNegativeInteger ;
            owl:onProperty uml:minDurationValue ],
        [ a owl:Restriction ;
            owl:minCardinality "1"^^xsd:nonNegativeInteger ;
            owl:onProperty uml:maxDurationValue ],
        [ a owl:Restriction ;
            owl:allValuesFrom uml:ValueSpecification ;
            owl:onProperty uml:minDurationValue ],
        [ a owl:Restriction ;
            owl:allValuesFrom uml:ValueSpecification ;
            owl:onProperty uml:maxDurationValue ],
        uml:Interval .

uml:TimeExpression a owl:Class ;
    rdfs:comment "A TimeExpression is a ValueSpecification that represents a time value." ;
    rdfs:subClassOf [ a owl:Restriction ;
            owl:allValuesFrom uml:ValueSpecification ;
            owl:onProperty uml:exprValue ],
        [ a owl:Restriction ;
            owl:maxCardinality "1"^^xsd:nonNegativeInteger ;
            owl:onProperty uml:exprValue ],
        [ a owl:Restriction ;
            owl:minCardinality "0"^^xsd:nonNegativeInteger ;
            owl:onProperty uml:exprValue ],
        [ a owl:Restriction ;
            owl:allValuesFrom uml:Observation ;
            owl:onProperty uml:observationValue ],
        uml:ValueSpecification .

uml:TimeInterval a owl:Class ;
    rdfs:comment "A TimeInterval defines the range between two TimeExpressions." ;
    rdfs:subClassOf [ a owl:Restriction ;
            owl:maxCardinality "1"^^xsd:nonNegativeInteger ;
            owl:onProperty uml:maxTimeValue ],
        [ a owl:Restriction ;
            owl:minCardinality "1"^^xsd:nonNegativeInteger ;
            owl:onProperty uml:minTimeValue ],
        [ a owl:Restriction ;
            owl:maxCardinality "1"^^xsd:nonNegativeInteger ;
            owl:onProperty uml:minTimeValue ],
        [ a owl:Restriction ;
            owl:allValuesFrom uml:ValueSpecification ;
            owl:onProperty uml:maxTimeValue ],
        [ a owl:Restriction ;
            owl:minCardinality "1"^^xsd:nonNegativeInteger ;
            owl:onProperty uml:maxTimeValue ],
        [ a owl:Restriction ;
            owl:allValuesFrom uml:ValueSpecification ;
            owl:onProperty uml:minTimeValue ],
        uml:Interval .

uml:lowerValue a owl:ObjectProperty ;
    rdfs:label "lower_value" ;
    rdfs:comment "For MultiplicityElement abstract class; UML 2.5.1 specification section 7.5" ;
    rdfs:domain sbol:Identified ;
    rdfs:range uml:ValueSpecification ;
    rdfs:subPropertyOf sbol:directlyComprises .

uml:upperValue a owl:ObjectProperty ;
    rdfs:label "upper_value" ;
    rdfs:comment "For MultiplicityElement abstract class; UML 2.5.1 specification section 7.5" ;
    rdfs:domain sbol:Identified ;
    rdfs:range uml:ValueSpecification ;
    rdfs:subPropertyOf sbol:directlyComprises .

uml:Observation a owl:Class ;
    rdfs:comment "Observation specifies a value determined by observing an event or events that occur relative to other model entities." ;
    rdfs:subClassOf sbol:Identified .

uml:ActivityEdge a owl:Class ;
    rdfs:comment "An ActivityEdge is an abstract class for directed connections between two ActivityNodes. See UML 2.5.1 specification section 15.2." ;
    rdfs:subClassOf [ a owl:Restriction ;
            owl:allValuesFrom uml:ActivityNode ;
            owl:onProperty uml:source ],
        [ a owl:Restriction ;
            owl:minCardinality "1"^^xsd:nonNegativeInteger ;
            owl:onProperty uml:source ],
        [ a owl:Restriction ;
            owl:maxCardinality "1"^^xsd:nonNegativeInteger ;
            owl:onProperty uml:source ],
        [ a owl:Restriction ;
            owl:allValuesFrom uml:ActivityNode ;
            owl:onProperty uml:target ],
        [ a owl:Restriction ;
            owl:minCardinality "1"^^xsd:nonNegativeInteger ;
            owl:onProperty uml:target ],
        [ a owl:Restriction ;
            owl:maxCardinality "1"^^xsd:nonNegativeInteger ;
            owl:onProperty uml:target ],
        sbol:Identified .

uml:Constraint a owl:Class ;
    rdfs:comment "A Constraint is a condition or restriction expressed in natural language text or in a machine readable language. See UML 2.5.1 specification section 7.6." ;
    rdfs:subClassOf [ a owl:Restriction ;
            owl:allValuesFrom uml:OrderedPropertyValue ;
            owl:onProperty uml:constrainedElement ],
        sbol:Identified .

uml:ControlNode a owl:Class ;
    rdfs:comment "A ControlNode is a kind of ActivityNode used to manage the flow of tokens between other nodes in an Activity. It can manage branching and merging of workflows and the implementation of logic for flow control. See UML 2.5.1 specification section 15.3." ;
    rdfs:subClassOf uml:ActivityNode .

uml:exprValue a owl:ObjectProperty ;
    rdfs:label "expr" ;
    rdfs:comment "A ValueSpecification that evaluates to the value of the Duration." ;
    rdfs:domain uml:Duration,
        uml:TimeExpression ;
    rdfs:range uml:ValueSpecification ;
    rdfs:subPropertyOf sbol:directlyComprises .

uml:isUnique a owl:DatatypeProperty ;
    rdfs:label "is_unique" ;
    rdfs:comment "For MultiplicityElement abstract class; UML 2.5.1 specification section 7.5" ;
    rdfs:domain sbol:Identified ;
    rdfs:range xsd:boolean .

uml:type a owl:DatatypeProperty ;
    rdfs:label "type" ;
    rdfs:comment "Specifies a set of Type instances constraining the allowed values. See UML 2.5.1 specification section 7.5." ;
    rdfs:domain sbol:Identified ;
    rdfs:range xsd:anyURI .

uml:LiteralSpecification a owl:Class ;
    rdfs:comment "A LiteralSpecification identifies a literal constant being modeled. See UML 2.5.1 specification section 8.2." ;
    rdfs:subClassOf uml:ValueSpecification .

uml:Behavior a owl:Class ;
    rdfs:comment "Behavior is an abstract specification of how a state changes over time. This specification may be a prospective definition of a protocol or a capture of an execution trace. See UML 2.5.1 specification section 13.2." ;
    rdfs:subClassOf [ a owl:Restriction ;
            owl:allValuesFrom uml:Constraint ;
            owl:onProperty uml:precondition ],
        [ a owl:Restriction ;
            owl:allValuesFrom uml:Constraint ;
            owl:onProperty uml:postcondition ],
        [ a owl:Restriction ;
            owl:allValuesFrom uml:OrderedPropertyValue ;
            owl:onProperty uml:ownedParameter ],
        sbol:TopLevel .

uml:ActivityNode a owl:Class ;
    rdfs:comment "ActivityNode is an abstract class for points in the flow of an Activity connected by ActivityEdges. See UML 2.5.1 specification section 15.2." ;
    rdfs:subClassOf sbol:Identified .

uml:isOrdered a owl:DatatypeProperty ;
    rdfs:label "is_ordered" ;
    rdfs:comment "For MultiplicityElement abstract class; UML 2.5.1 specification section 7.5" ;
    rdfs:domain sbol:Identified ;
    rdfs:range xsd:boolean .

uml:firstEventValue a owl:ObjectProperty ;
    rdfs:label "firstEvent" ;
    rdfs:comment "The value of firstEvent[i] is related to event[i] (where i is 1 or 2). If firstEvent[i] is true, then the correspondingobservation event is the first time instant the execution enters event[i]. If firstEvent[i] is false, then the corresponding observation event is the time instant the execution exits event[i]." ;
    rdfs:domain uml:DurationConstraint,
        uml:DurationObservation,
        uml:TimeConstraint,
        uml:TimeObservation ;
    rdfs:range uml:OrderedPropertyValue ;
    rdfs:subPropertyOf sbol:directlyComprises .

uml:OrderedPropertyValue a owl:Class ;
    rdfs:subClassOf [ a owl:Restriction ;
            owl:maxCardinality "1"^^xsd:nonNegativeInteger ;
            owl:onProperty uml:indexValue ],
        [ a owl:Restriction ;
            owl:allValuesFrom sbol:Identified ;
            owl:onProperty uml:propertyValue ],
        [ a owl:Restriction ;
            owl:minCardinality "1"^^xsd:nonNegativeInteger ;
            owl:onProperty uml:indexValue ],
        [ a owl:Restriction ;
            owl:allValuesFrom xsd:integer ;
            owl:onProperty uml:indexValue ],
        [ a owl:Restriction ;
            owl:maxCardinality "1"^^xsd:nonNegativeInteger ;
            owl:onProperty uml:propertyValue ],
        [ a owl:Restriction ;
            owl:minCardinality "1"^^xsd:nonNegativeInteger ;
            owl:onProperty uml:propertyValue ],
        sbol:Identified .

uml:ValueSpecification a owl:Class ;
    rdfs:label "ValueSpecification" ;
    rdfs:comment "A ValueSpecification is the specification of a (possibly empty) set of values. See UML 2.5.1 specification section 8." ;
    rdfs:subClassOf [ a owl:Restriction ;
            owl:allValuesFrom xsd:anyURI ;
            owl:onProperty uml:type ],
        [ a owl:Restriction ;
            owl:maxCardinality "1"^^xsd:nonNegativeInteger ;
            owl:onProperty uml:type ],
        sbol:Identified .

sbol:directlyComprises a owl:ObjectProperty .
